src/lib/kernel/gemm/Kuiper.Kernel.GEMM.TensorCore2D.To.KernelDesc.EpilogueStep.fsti
@@ -6,6 +6,8 @@ open Kuiper
 #set-options "--ifuel 1 --initial_fuel 0 --max_fuel 1"
 #set-options "--z3rlimit 15 --split_queries always"
 
+open Kuiper.Array.Vectorized { has_vec_cpy, chunk }
+open Kuiper.Array2.Strided
 open Kuiper.EMatrix
 open Kuiper.Tensor
 open Kuiper.Tensor.Layout.Alg { l2_row_major as rm }
@@ -14,22 +16,24 @@ open Pulse.Lib.Array
 
 module SZ = Kuiper.SizeT
 module T = Kuiper.Tensor
+module VG = Kuiper.Array2.Vectorized.Group
 
 open Kuiper.Kernel.GEMM.TensorCore2D.To.KernelDesc
 open Kuiper.Kernel.GEMM.TensorCore2D.To.KernelDesc.EpilogueCellUpdate
 
 let lane_coincide
-  (#et : Type0) {| scalar et |}
+  (#et : Type0) {| scalar et, hvc : has_vec_cpy et |}
   (#rows #cols : nat)
   (lane : natlt warp_size)
   (em1 em2 : chest2 et rows cols)
   : prop
 = forall (i : natlt rows) (j : natlt cols).
-    in_lane rows cols lane (i, j) ==> acc2 em1 i j == acc2 em2 i j
+    in_lane (chunk et #_ #hvc) rows cols lane (i, j) ==>
+      acc2 em1 i j == acc2 em2 i j
 
 ghost
 fn own_lane_cells_rw
-  (#et : Type0) {| scalar et |}
+  (#et : Type0) {| scalar et, hvc : has_vec_cpy et |}
   (#rows #cols : nat)
   (#l : layout2 rows cols)
   (m : array2 et l)
@@ -38,61 +42,53 @@ fn own_lane_cells_rw
   (#_ : squash (lane_coincide lane em1 em2))
   requires own_lane_cells m em1 lane
   ensures own_lane_cells m em2 lane
+
+(* [em0] with the chunk groups of [lane] whose index is below [upto]
+   replaced by their values in [em1]. *)
 let lane_fade
-  (#et : Type0) {| scalar et |}
+  (#et : Type0) {| scalar et, hvc : has_vec_cpy et |}
   (#rows #cols : pos)
   (em0 em1 : chest2 et rows cols)
   (lane : natlt warp_size)
   (upto : nat)
   : chest2 et rows cols
 = mk2 (fun i j ->
-    let flat = i * cols + j in
-    if in_lane rows cols lane (i, j) && flat < upto
+    if in_lane (chunk et #_ #hvc) rows cols lane (i, j)
+       && VG.group_of (chunk et #_ #hvc) cols i j < upto
     then acc2 em1 i j
     else acc2 em0 i j)
 
 let lane_fade_start
-  (#et : Type0) {| scalar et |}
+  (#et : Type0) {| scalar et, hvc : has_vec_cpy et |}
   (#rows #cols : pos)
   (em0 em1 : chest2 et rows cols)
   (lane : natlt warp_size)
   : Lemma (lane_coincide lane em0 (lane_fade em0 em1 lane lane))
 = ()
 
-let lane_fade_step
-  (#et : Type0) {| scalar et |}
-  (#rows #cols : pos)
-  (em0 em1 : chest2 et rows cols)
-  (lane : natlt warp_size)
-  (flat : nat{flat < rows * cols /\ flat % warp_size == lane})
-  : Lemma (
-      let row = flat / cols in
-      let col = flat % cols in
-      lane_coincide lane
-        (upd2 (lane_fade em0 em1 lane flat) row col (acc2 em1 row col))
-        (lane_fade em0 em1 lane (flat + warp_size)))
-= ()
-
 let lane_fade_done
-  (#et : Type0) {| scalar et |}
+  (#et : Type0) {| scalar et, hvc : has_vec_cpy et |}
   (#rows #cols : pos)
   (em0 em1 : chest2 et rows cols)
   (lane : natlt warp_size)
-  (upto : nat{rows * cols <= upto})
-  : Lemma (lane_coincide lane (lane_fade em0 em1 lane upto) em1)
+  (upto : nat{VG.ngroups (chunk et #_ #hvc) rows cols <= upto})
+  : Lemma (requires chunk et #_ #hvc /?+ cols)
+          (ensures lane_coincide lane (lane_fade em0 em1 lane upto) em1)
 = ()
 
 inline_for_extraction noextract
 fn epilogue_fragment_step
   (#et_cd #et_acc : Type0)
-  {| scalar et_cd, scalar et_acc |}
+  {| scalar et_cd, hvc : has_vec_cpy et_cd, scalar et_acc |}
   (comb : et_cd -> et_acc -> et_cd)
   (#m #n : szp)
+  {| str : strided_row_major (rm m n) |}
   (c : array2 et_cd (rm m n))
   (#_ : squash (SZ.fits (m * n)))
   (bm bn rows cols wm wn : szp)
   (#_ : squash (bm /?+ m /\ bn /?+ n /\
                 wm * rows /?+ bm /\ wn * cols /?+ bn))
+  (#_ : squash (chunk et_cd /?+ cols))
   (mrow : szlt (m / bm))
   (mcol : szlt (n / bn))
   (warpRow : szlt (bm / (wm * rows)))
@@ -120,23 +116,25 @@ fn epilogue_fragment_step
       bm bn rows cols wm wn
       (SZ.v mrow) (SZ.v mcol) (SZ.v warpRow) (SZ.v warpCol)
       (SZ.v idx) eAcc))
-  (vf : sz{
-    SZ.v vf < rows * cols /\
-    SZ.v vf % warp_size == lane /\
-    SZ.v vf <= rows * cols + warp_size})
+  (vg : sz{
+    SZ.v vg < VG.ngroups (chunk et_cd) rows cols /\
+    SZ.v vg % warp_size == lane})
   preserves
     gpu **
     c |-> Frac fC eC **
     acc |-> Frac (1.0R /. warp_size) eAcc
   requires
+    pure (aligned 16 (T.core c) /\ aligned 16 (T.core d) /\
+          aligned_strided_row_major (chunk et_cd) str)
+  requires
     own_lane_cells
       (output_fragment d bm bn rows cols wm wn
         (SZ.v bid) (SZ.v wid) (SZ.v idx / wn) (SZ.v idx % wn))
-      (lane_fade eD0 eTarget lane vf)
+      (lane_fade eD0 eTarget lane vg)
       lane
   ensures
     own_lane_cells
       (output_fragment d bm bn rows cols wm wn
         (SZ.v bid) (SZ.v wid) (SZ.v idx / wn) (SZ.v idx % wn))
-      (lane_fade eD0 eTarget lane (SZ.v vf + warp_size))
+      (lane_fade eD0 eTarget lane (SZ.v vg + warp_size))
       lane
