src/lib/kernel/gemm/Kuiper.Kernel.GEMM.TensorCore2D.To.EpilogueLoopStep.fsti
@@ -3,13 +3,16 @@ module Kuiper.Kernel.GEMM.TensorCore2D.To.EpilogueLoopStep
 #lang-pulse
 
 open Kuiper
+open Kuiper.Array.Vectorized { has_vec_cpy, chunk }
 open Kuiper.EMatrix
 open Kuiper.Tensor
+open Kuiper.Array2.Strided
 open Kuiper.Tensor.Layout.Alg { l2_row_major as rm }
 open Kuiper.TensorCore
 open Pulse.Lib.Array
 
 module SZ = Kuiper.SizeT
+module T = Kuiper.Tensor
 
 open Kuiper.Kernel.GEMM.TensorCore2D.KernelDesc
 open Kuiper.Kernel.GEMM.TensorCore2D.To.KernelDesc
@@ -19,11 +22,12 @@ open Kuiper.Kernel.GEMM.TensorCore2D.To.EpilogueState
 inline_for_extraction noextract
 fn epilogue_loop_step
   (#et_ab #et_cd #et_acc : Type0)
-  {| scalar et_ab, scalar et_cd, real_like et_cd,
+  {| scalar et_ab, scalar et_cd, real_like et_cd, has_vec_cpy et_cd,
      scalar et_acc, real_like et_acc |}
   (comb : et_cd -> et_acc -> et_cd)
   (comb_r : binop real { approx2 comb comb_r })
   (#m #n : szp)
+  {| str : strided_row_major (rm m n) |}
   (gC : array2 et_cd (rm m n))
   (#fC : perm)
   (#eC : chest2 et_cd m n)
@@ -39,6 +43,7 @@ fn epilogue_loop_step
     SZ.v nthr == bm / (wm * tm) * (bn / (wn * tn)) * warp_size })
   (#_ : squash (SZ.fits ((nthr / warp_size) * tm * tn)))
   (#_ : squash (SZ.fits (tm * tn + warp_size)))
+  (#_ : squash (chunk et_cd /?+ tn))
   (sh : c_shmems
     (shmems_desc_to et_ab et_acc bm bn bk tm tn nthr))
   (accFrags : array
@@ -59,6 +64,8 @@ fn epilogue_loop_step
   (done : szle (wm * wn) { SZ.v done < wm * wn })
   norewrite
   requires
+    pure (aligned 16 (T.core gC) /\ aligned 16 (T.core gD) /\
+          aligned_strided_row_major (chunk et_cd) str) **
     idx |-> done **
     epilogue_frame #et_ab #et_cd #et_acc
       #_ #_ #_ #_ #_
@@ -70,6 +77,8 @@ fn epilogue_loop_step
       (chest_comb comb_r rCWarp rAcc)
       (SZ.v done)
   ensures
+    pure (aligned 16 (T.core gC) /\ aligned 16 (T.core gD) /\
+          aligned_strided_row_major (chunk et_cd) str) **
     (exists* (next : szle (wm * wn)).
       idx |-> next **
       pure (SZ.v next == SZ.v done + 1)) **
